

Spring 2020 - Knowledge Discovery in Data at Scale Technologies - Homework #4

by Almaz Murzabekov

Homework description

Optimal Estimation

Consider the following series of measurements of the unknown value x :

$$y_i = a_i x + \varepsilon_i, \quad i = 1, \dots, n,$$

where y_i are measurement results, a_i are known coefficients, and ε_i represent random error of measurement and are independent identically distributed (i.i.d.) with zero mean and variance σ^2 :

$$E\varepsilon_i = 0, E\varepsilon_i^2 = \sigma^2, \quad i = 1, \dots, n$$

a) What function of y_1, \dots, y_n (and of a_1, \dots, a_n) would you use as a good estimate \hat{x} for x ? $\hat{x} = ?$

(Hint: try best linear estimate or least squares estimate).

Estimation of x might be formulated in the following formula, and the value of this formula we should minimize

$$Q(x) = \sum_{i=1}^n \frac{(y_i - a_i x)^2}{\sigma^2} \rightarrow \min$$

$$\frac{dQ}{dx} = \sum_{i=1}^n \frac{(-2y_i a_i + 2a_i^2 x)}{\sigma^2} = \sum_{i=1}^n \frac{-2(y_i a_i - a_i^2 x)}{\sigma^2} = -2 \sum_{i=1}^n \frac{y_i a_i - a_i^2 x}{\sigma^2} = 0 \Rightarrow$$

$$-2 \sum_{i=1}^n \frac{y_i a_i - a_i^2 x}{\sigma^2} = 0 \Rightarrow$$

$$-2 \left(\sum_{i=1}^n \frac{y_i a_i}{\sigma^2} - \sum_{i=1}^n \frac{a_i^2 x}{\sigma^2} \right) = 0 \Rightarrow$$

$$-2 \neq 0 \Rightarrow \left(\sum_{i=1}^n \frac{y_i a_i}{\sigma^2} - \sum_{i=1}^n \frac{a_i^2 x}{\sigma^2} \right) = 0 \Rightarrow$$

$$\left(\sum_{i=1}^n \frac{y_i a_i}{\sigma^2} - \sum_{i=1}^n \frac{a_i^2 x}{\sigma^2} \right) = 0 \Rightarrow$$

$$\sum_{i=1}^n \frac{y_i a_i}{\sigma^2} = \sum_{i=1}^n \frac{a_i^2 x}{\sigma^2} \Rightarrow (*\sigma^2)$$

$$\sum_{i=1}^n y_i a_i = \sum_{i=1}^n a_i^2 x \Rightarrow$$

$$\sum_{i=1}^n y_i a_i = x \sum_{i=1}^n a_i^2 \Rightarrow$$

$$x \sum_{i=1}^n a_i^2 = \sum_{i=1}^n y_i a_i \Rightarrow$$

$$\hat{x} = \frac{\sum_{i=1}^n y_i a_i}{\sum_{i=1}^n a_i^2}$$

b) Is this estimate optimal in any sense?

In this work I'm using the method **Least squares estimate**. This method/function approximation applies the principle of least squares to function approximation, by means of a weighted sum of other functions. The best approximation can be defined as that which minimises the difference between the original function and the approximation; for a least-squares approach the quality of the approximation is measured in terms of the squared differences between the two.

c) Is it a biased or an unbiased estimate?

$$\hat{x} = \frac{\sum_{i=1}^n y_i a_i}{\sum_{i=1}^n a_i^2} \rightarrow E(\hat{x}) = ?$$

$$E(\hat{x}) = E\left(\frac{\sum_{i=1}^n y_i a_i}{\sum_{i=1}^n a_i^2}\right) \Rightarrow \quad \text{where} \quad y_i = a_i x + \varepsilon_i,$$

$$E(\hat{x}) = E\left(\frac{\sum_{i=1}^n a_i(a_i x + \varepsilon_i)}{\sum_{i=1}^n a_i^2}\right) \Rightarrow$$

$$E(\hat{x}) = E\left(\frac{\sum_{i=1}^n a_i^2 x + a_i \varepsilon_i}{\sum_{i=1}^n a_i^2}\right) \Rightarrow \quad E(\varepsilon_i) = 0$$

$$E(\hat{x}) = E\left(\frac{\sum_{i=1}^n a_i^2 x}{\sum_{i=1}^n a_i^2}\right) \Rightarrow \quad \text{where } x - \text{is constant}$$

$$E(\hat{x}) = E\left(\frac{x \sum_{i=1}^n a_i^2}{\sum_{i=1}^n a_i^2}\right) \Rightarrow$$

$$E(\hat{x}) = E(x) = x$$

that means, this is **unbiased** estimation

d) What is its variance (expressed through σ^2)? $Var(\hat{x}) = ?$

$$Var(\hat{x}) = E(\hat{x} - x)^2 \Rightarrow$$

$$Var(\hat{x}) = E\left(\frac{\sum_{i=1}^n y_i a_i}{\sum_{i=1}^n a_i^2} - x\right)^2 \Rightarrow \quad \text{where} \quad y_i = a_i x + \varepsilon_i,$$

$$Var(\hat{x}) = E\left(\frac{\sum_{i=1}^n a_i(a_i x + \varepsilon_i)}{\sum_{i=1}^n a_i^2} - x\right)^2 \Rightarrow$$

$$Var(\hat{x}) = E\left(\frac{\sum_{i=1}^n a_i^2 x + a_i \varepsilon_i}{\sum_{i=1}^n a_i^2} - x\right)^2 \Rightarrow$$

$$Var(\hat{x}) = E\left(\frac{\sum_{i=1}^n a_i^2 x + \sum_{i=1}^n a_i \varepsilon_i}{\sum_{i=1}^n a_i^2} - x\right)^2 \Rightarrow$$

$$Var(\hat{x}) = E\left(\frac{\sum_{i=1}^n a_i^2 x}{\sum_{i=1}^n a_i^2} + \frac{\sum_{i=1}^n a_i \varepsilon_i}{\sum_{i=1}^n a_i^2} - x\right)^2 \Rightarrow$$

$$Var(\hat{x}) = E\left(x + \frac{\sum_{i=1}^n a_i \varepsilon_i}{\sum_{i=1}^n a_i^2} - x\right)^2 \Rightarrow$$

$$Var(\hat{x}) = E\left(\frac{\sum_{i=1}^n a_i \varepsilon_i}{\sum_{i=1}^n a_i^2}\right)^2 \Rightarrow$$

$$Var(\hat{x}) = E\left(\frac{\sum_{i=1}^n (a_i \varepsilon_i)^2}{(\sum_{i=1}^n a_i^2)^2}\right) \Rightarrow$$

$$Var(\hat{x}) = E\left(\frac{\sum_{i,j=1}^n a_i a_j \varepsilon_i \varepsilon_j}{(\sum_{i=1}^n a_i^2)^2}\right) \Rightarrow$$

$$Var(\hat{x}) = \frac{\sum_{i,j=1}^n a_i a_j E(\varepsilon_i \varepsilon_j)}{(\sum_{i=1}^n a_i^2)^2} \Rightarrow$$

$$E\hat{x} = \begin{cases} 0 & \text{if } i \neq j \\ \sigma^2 & \text{if } i = j \end{cases}$$

$$Var(\hat{x}) = \frac{\sigma^2 \sum_{i=1}^n a_i^2}{(\sum_{i=1}^n a_i^2)^2} \Rightarrow$$

$$Var(\hat{x}) = \frac{\sigma^2}{\sum_{i=1}^n a_i^2}$$

e) How would you estimate σ^2 if it is unknown? $\hat{\sigma}^2 = ?$

$$\text{Var}(\varepsilon) = E[(\varepsilon - E(\varepsilon))^2] \quad E(\varepsilon) = 0, \Rightarrow$$

$$\text{Var}(\varepsilon) = E[(\varepsilon)^2] = \sigma^2 \Rightarrow$$

$$E\left(\sum_{i=1}^n (y_i - a_i x)^2\right) = \quad \text{where } y_i = a_i x + \varepsilon_i$$

$$E \sum_{i=1}^n (a_i x + \varepsilon_i - a_i x)^2 = E \sum_{i=1}^n (\varepsilon_i)^2 = n\sigma^2$$

$$\widehat{\sigma^2} = \frac{\sum_{i=1}^n (y_i - a_i \hat{x})^2}{n} \Rightarrow$$

$$\widehat{\sigma^2} = \frac{\sum_{i=1}^n (y_i^2 - 2a_i y_i \hat{x} + a_i^2 \hat{x}^2)}{n} \Rightarrow$$

$$\widehat{\sigma^2} = \frac{\sum_{i=1}^n y_i^2 - \sum_{i=1}^n 2a_i y_i \hat{x} + \sum_{i=1}^n a_i^2 \hat{x}^2}{n} \Rightarrow$$

$$\widehat{\sigma^2} = \frac{\sum_{i=1}^n y_i^2 - 2\hat{x} \sum_{i=1}^n a_i y_i + \hat{x}^2 \sum_{i=1}^n a_i^2}{n} \Rightarrow \quad \text{considering that } \hat{x} = \frac{\sum_{i=1}^n y_i a_i}{\sum_{i=1}^n a_i^2}$$

$$\widehat{\sigma^2} = \frac{\sum_{i=1}^n y_i^2 - 2 \frac{\sum_{i=1}^n y_i a_i}{\sum_{i=1}^n a_i^2} \sum_{i=1}^n a_i y_i + \left(\frac{\sum_{i=1}^n y_i a_i}{\sum_{i=1}^n a_i^2}\right)^2 \sum_{i=1}^n a_i^2}{n} \Rightarrow$$

$$\widehat{\sigma^2} = \frac{\sum_{i=1}^n y_i^2 - 2 \frac{(\sum_{i=1}^n y_i a_i)^2}{\sum_{i=1}^n a_i^2} + \frac{\sum_{i=1}^n (y_i a_i)^2}{\sum_{i=1}^n a_i^2}}{n}$$

$$\widehat{\sigma^2} = \frac{\sum_{i=1}^n y_i^2 - \frac{\sum_{i=1}^n (y_i a_i)^2}{\sum_{i=1}^n a_i^2}}{n} \Rightarrow \text{biased estimation}$$

$$\widehat{\sigma^2} = \frac{\sum_{i=1}^n y_i^2 - \frac{\sum_{i=1}^n (y_i a_i)^2}{\sum_{i=1}^n a_i^2}}{n-1} \Rightarrow \text{unbiased estimation}$$

f) What would you use as an estimate for $Var(\hat{x})$ if σ^2 is unknown? $\widehat{Var}(\hat{x}) = ?$

$$Var(\hat{x}) = \frac{\sigma^2}{\sum_{i=1}^n a_i^2} \Rightarrow \text{considering that } \sigma^2 =$$

$$\widehat{\sigma^2} = \frac{\sum_{i=1}^n y_i^2 - \frac{\sum_{i=1}^n (y_i a_i)^2}{\sum_{i=1}^n a_i^2}}{n-1}$$

$$\widehat{Var}(\hat{x}) = \frac{\sum_{i=1}^n y_i^2 - \frac{\sum_{i=1}^n (y_i a_i)^2}{\sum_{i=1}^n a_i^2}}{(n-1)(\sum_{i=1}^n a_i^2)}$$

g) Suppose that the variance σ^2 is known. What "canonical information" would be sufficient to extract from the series of records

$$(y_1, a_1), \dots, (y_n, a_n), \quad i = 1, \dots, n$$

\ in order to compute the estimate \hat{x} , and its variance $Var(\hat{x})$?

$$\hat{x} = \frac{\sum_{i=1}^n y_i a_i}{\sum_{i=1}^n a_i^2} \quad Var(\hat{x}) = \frac{\sigma^2}{\sum_{i=1}^n a_i^2}$$

$$T = \sum_{i=1}^n a_i y_i; \quad V = \sum_{i=1}^n a_i^2;$$

$$\hat{x} = \frac{T}{V}; \quad Var(\hat{x}) = \frac{\sigma^2}{V}$$

h) Suppose that the variance σ^2 is NOT known. What "canonical information" would be sufficient to extract from the series of observations in order to compute \hat{x} , $\widehat{\sigma^2}$, and $\widehat{Var}(\hat{x})$?

$$T = \sum_{i=1}^n a_i y_i; \quad V = \sum_{i=1}^n a_i^2; \quad Z = \sum_{i=1}^n y_i^2;$$

$$Q = \sum_{i=1}^n (a_i y_i)^2; \quad N = \text{Number of observation}$$

$$\hat{x} = \frac{\sum_{i=1}^n y_i a_i}{\sum_{i=1}^n a_i^2} = \frac{T}{V}$$

$$\widehat{\sigma^2} = \frac{\sum_{i=1}^n y_i^2 - \frac{\sum_{i=1}^n (y_i a_i)^2}{\sum_{i=1}^n a_i^2}}{n-1} = \frac{Z - \frac{Q}{V}}{N-1}$$

$$\widehat{Var(\hat{x})} = \frac{\sum_{i=1}^n y_i^2 - \frac{\sum_{i=1}^n (y_i a_i)^2}{\sum_{i=1}^n a_i^2}}{(n-1)(\sum_{i=1}^n a_i^2)} = \frac{Z - \frac{Q}{V}}{(N-1)V}$$

i) How should we update such "information" when a new record (y_{n+1}, a_{n+1}) arrives?

Case when σ^2 is known

$$(T_1, V_1) \oplus (y_{n+1}, a_{n+1}) = ($$

$$T_1 + y_{n+1} a_{n+1},$$

$$V_1 + a_{n+1}^2)$$

Case when σ^2 is unknown

$$(T_1, V_1, Z_1, Q_1, N_1) \oplus (y_{n+1}, a_{n+1}) = ($$

$$T_1 + y_{n+1} a_{n+1},$$

$$V_1 + a_{n+1}^2,$$

$$Z_1 + y_{n+1}^2,$$

$$Q_1 + (y_{n+1} a_{n+1})^2,$$

$$N_1 + 1)$$

j) How should we "combine" (merge) two pieces of "canonical information"?

Case when σ^2 is known

$$(T_1, V_1) \oplus (T_2, V_2) = (T_1 + T_2, V_1 + V_2)$$

Case when σ^2 is unknown

$$(T_1, V_1, Z_1, Q_1, N_1) \oplus (T_2, V_2, Z_2, Q_2, N_2) = \\ (T_1 + T_2, V_1 + V_2, Z_1 + Z_2, Q_1 + Q_2, N_1 + N_2)$$
